tests/lowparse/TestPair.fst
@@ -6,8 +6,8 @@ module LM = LowParseExampleMono
 module LMI = LowParse.Low.Int
 
 assume val buf :
-  s: LM.slice{
-    FB.recallable s.LM.base
+  s: FB.buffer {
+    FB.recallable s
   }
 let irepr #t #k (p:LM.parser k t) = LM.irepr p buf
 
@@ -39,14 +39,14 @@ let read_components2 (i:irepr P.pair_parser)
       True)
   = LM.recall_valid i;
     let x = P.accessor_pair_fst buf (LM.irepr_pos i) in
-    FB.recall_frozen_until_default buf.LM.base;
+    FB.recall_frozen_until_default buf;
     let x : irepr LPI.parse_u32 = LM.witness_valid buf x in
 
     havoc();
 
     LM.recall_valid i;
     let y : UInt32.t = P.accessor_pair_snd buf (LM.irepr_pos i) in
-    FB.recall_frozen_until_default buf.LM.base;
+    FB.recall_frozen_until_default buf;
     assert (UInt32.v y >= 4);
     let y : irepr LPI.parse_u16 = LM.witness_valid buf y in
     x, y
@@ -65,30 +65,30 @@ let read_components3 (i:irepr P.pair_parser)
 module HS = FStar.HyperStack
 module U32 = FStar.UInt32
 
-let frozen_until = LM.buffer_frozen_until buf.LM.base
+let frozen_until = LM.buffer_frozen_until buf
 
 let iwrite_u16 (u:UInt16.t) (p:UInt32.t)
   : Stack (irepr LPI.parse_u16)
     (requires fun h ->
       frozen_until h <= U32.v p /\
-      U32.v p + 2 < U32.v buf.LM.len)
+      U32.v p + 2 < B.length buf)
     (ensures fun h0 i h1 ->
       LM.irepr_pos i == p /\
       LM.irepr_pos' i == U32.(p +^ 2ul) /\
       LM.irepr_v i == u   /\
       frozen_until h1 == U32.v p + 2 /\
-      B.modifies (B.loc_buffer buf.LM.base) h0 h1)
-   = FB.recall_frozen_until_default buf.LM.base;
-     B.recall buf.LM.base;
+      B.modifies (B.loc_buffer buf) h0 h1)
+   = FB.recall_frozen_until_default buf;
+     B.recall buf;
      let h0 = get () in
      let p' = LMI.write_u16 u buf p in
      let h1 = get () in
      let p' = p `U32.add` 2ul in
-     B.modifies_buffer_from_to_elim buf.LM.base 0ul 4ul (LM.loc_slice_from_to buf p p') h0 h1;
-     FB.recall_frozen_until_default buf.LM.base;
-     FB.freeze buf.LM.base p' ;
+     B.modifies_buffer_from_to_elim buf 0ul 4ul (B.loc_buffer_from_to buf p p') h0 h1;
+     FB.recall_frozen_until_default buf;
+     FB.freeze buf p' ;
      let h2 = get () in
-     LM.valid_exact_ext_intro LPI.parse_u16 h1 buf p p' h2 buf p p' ;
+     LM.valid_exact_ext_intro LPI.parse_u16 h1 (LM.slice_of_buffer buf) p p' h2 (LM.slice_of_buffer buf) p p' ;
      LM.witness_valid buf p
 
 
@@ -96,24 +96,24 @@ let iwrite_u32 (u:UInt32.t) (p:UInt32.t)
   : Stack (irepr LPI.parse_u32)
     (requires fun h ->
       frozen_until h <= U32.v p /\
-      U32.v p + 4 < U32.v buf.LM.len)
+      U32.v p + 4 < B.length buf)
     (ensures fun h0 i h1 ->
       LM.irepr_pos i == p /\
       LM.irepr_pos' i == U32.(p +^ 4ul) /\
       LM.irepr_v i == u   /\
       frozen_until h1 == U32.v p + 4 /\
-      B.modifies (B.loc_buffer buf.LM.base) h0 h1)
-   = FB.recall_frozen_until_default buf.LM.base;
-     B.recall buf.LM.base;
+      B.modifies (B.loc_buffer buf) h0 h1)
+   = FB.recall_frozen_until_default buf;
+     B.recall buf;
      let h0 = get () in
      let p' = LMI.write_u32 u buf p in
      let h1 = get () in
      let p' = p `U32.add` 4ul in
-     B.modifies_buffer_from_to_elim buf.LM.base 0ul 4ul (LM.loc_slice_from_to buf p p') h0 h1;
-     FB.recall_frozen_until_default buf.LM.base;
-     FB.freeze buf.LM.base p' ;
+     B.modifies_buffer_from_to_elim buf 0ul 4ul (B.loc_buffer_from_to buf p p') h0 h1;
+     FB.recall_frozen_until_default buf;
+     FB.freeze buf p' ;
      let h2 = get () in
-     LM.valid_exact_ext_intro LPI.parse_u32 h1 buf p p' h2 buf p p' ;
+     LM.valid_exact_ext_intro LPI.parse_u32 h1 (LM.slice_of_buffer buf) p p' h2 (LM.slice_of_buffer buf) p p' ;
      LM.witness_valid buf p
 
 assume val havoc_l :
@@ -127,20 +127,20 @@ let iwrite_pair (u0:UInt32.t) (u1:UInt16.t) (p:UInt32.t)
   : Stack (irepr P.pair_parser)
     (requires fun h ->
       frozen_until h <= U32.v p /\
-      U32.v p + 6 < U32.v buf.LM.len)
+      U32.v p + 6 < B.length buf)
     (ensures fun h0 i h1 ->
       LM.irepr_pos i == p /\
       LM.irepr_pos' i == U32.(p +^ 6ul) /\
       LM.irepr_v i == P.({fst=u0; snd=u1})  /\
       frozen_until h1 == U32.v p + 6 /\
-      B.modifies (B.loc_union some_loc (B.loc_buffer buf.LM.base)) h0 h1)
+      B.modifies (B.loc_union some_loc (B.loc_buffer buf)) h0 h1)
    = let i0 = iwrite_u32 u0 p in
      havoc_l some_loc;
      let i1 = iwrite_u16 u1 U32.(p +^ 4ul) in
      let h = get () in
      LM.recall_valid i0;
      LM.recall_valid i1;
-     Pair.pair_valid h buf p;
+     Pair.pair_valid h (LM.slice_of_buffer buf) p;
      LM.witness_valid buf p
 
 (* with the iwrite wrapper *)
@@ -149,20 +149,20 @@ let iwrite_pair1 (u0:UInt32.t) (u1:UInt16.t) (p:UInt32.t)
   : Stack (irepr P.pair_parser)
     (requires fun h ->
       frozen_until h <= U32.v p /\
-      U32.v p + 6 < U32.v buf.LM.len)
+      U32.v p + 6 < B.length buf)
     (ensures fun h0 i h1 ->
       LM.irepr_pos i == p /\
       LM.irepr_pos' i == U32.(p +^ 6ul) /\
       LM.irepr_v i == P.({fst=u0; snd=u1})  /\
       frozen_until h1 == U32.v p + 6 /\
-      B.modifies (B.loc_union some_loc (B.loc_buffer buf.LM.base)) h0 h1)
+      B.modifies (B.loc_union some_loc (B.loc_buffer buf)) h0 h1)
    = let i0 = LM.iwrite LMI.write_u32 u0 buf p in
      havoc_l some_loc;
      let i1 = LM.iwrite LMI.write_u16 u1 buf U32.(p +^ 4ul) in
      let h = get () in
      LM.recall_valid i0;
      LM.recall_valid i1;
-     Pair.pair_valid h buf p;
+     Pair.pair_valid h (LM.slice_of_buffer buf) p;
      LM.witness_valid buf p
 
 (* with only one freeze, thanks to frozen_until_frame that preserves the value of the length header across LowParse writers *)
@@ -171,17 +171,17 @@ let iwrite_pair2 (u0:UInt32.t) (u1:UInt16.t) (p:UInt32.t)
   : Stack (irepr P.pair_parser)
     (requires fun h ->
       frozen_until h <= U32.v p /\
-      U32.v p + 6 < U32.v buf.LM.len)
+      U32.v p + 6 < B.length buf)
     (ensures fun h0 i h1 ->
       LM.irepr_pos i == p /\
       LM.irepr_pos' i == U32.(p +^ 6ul) /\
       LM.irepr_v i == P.({fst=u0; snd=u1})  /\
       frozen_until h1 == U32.v p + 6 /\
-      B.modifies (B.loc_union some_loc (B.loc_buffer buf.LM.base)) h0 h1)
-= FB.recall_frozen_until_default buf.LM.base; // for writable
-  B.recall buf.LM.base; // for live
+      B.modifies (B.loc_union some_loc (B.loc_buffer buf)) h0 h1)
+= FB.recall_frozen_until_default buf; // for writable
+  B.recall buf; // for live
   let p1 = LMI.write_u32 u0 buf p in
   let p2 = LMI.write_u16 u1 buf p1 in
   let h = get () in
-  Pair.pair_valid h buf p;
+  Pair.pair_valid h (LM.slice_of_buffer buf) p;
   LM.freeze_valid Pair.pair_parser buf p p2
